# merged from LoLa and https://github.com/API4KBs/api4kbs/raw/master/ontologies/OntoIOpTerminology.rdf

Prefix: : <http://www.omg.org/spec/DOL/dol-language/>
Prefix: rdf: <http://www.w3.org/1999/02/22-rdf-syntax-ns#>
Prefix: rdfs: <http://www.w3.org/2000/01/rdf-schema#>
Prefix: owl: <http://www.w3.org/2002/07/owl#>
Prefix: xsd: <http://www.w3.org/2001/XMLSchema#>
Prefix: dct: <http://purl.org/dc/terms/>
Prefix: skos: <http://www.w3.org/2004/02/skos/core#>
Prefix: sm: <http://www.omg.org/techprocess/ab/SpecificationMetadata/>
Prefix: dol: <http://www.omg.org/spec/DOL/dol-language/>
	
# We can't use the non-standard community ontology OMV in an OMG standard
# Prefix: omv: <http://omv.ontoware.org/2005/05/ontology#>

Ontology: <http://www.omg.org/spec/DOL/dol-language/> <http://www.omg.org/spec/DOL/20150801/dol-language/>

Import: <http://www.omg.org/techprocess/ab/SpecificationMetadata/>

    Annotations: 
        owl:versionInfo "1.0",
        rdfs:comment "RDF serialization of DOL, implemented as an OWL ontology.  Actually some axioms that we would like to have go beyond OWL."@en,
        rdfs:comment "Developers' note: When scaling this ontology implementation up to DOL, look below for annotations marked as 'beyond OWL'.  These things can be modeled in FOL."@en,
        rdfs:seeAlso <http://www.informatik.uni-bremen.de/~till/papers/womo2012.pdf>,
        # omv:hasFormalityLevel <http://omv.ontoware.org/2005/05/ontology#Vocabulary>,
        # ^ actually this ontology is now more expressive than a vocabulary; plus, we can't use OMV
        # omv:conformsToKnowledgeRepresentationParadigm <http://omv.ontoware.org/2005/05/ontology#DescriptionLogics>,
        # ^ we can't use OMV; however "logic = description logic" should be clear from the fact that this is an OWL ontology
        # omv:isOfType <http://omv.ontoware.org/2005/05/ontology#DomainOntology>,
        # ^ we can't use OMV, and "domain ontology" is not quite right anyway.
		
	sm:copyright "Copyright (c) 2014-2015 Object Management Group, Inc.
Copyright (c) 2014-2015 Thematix Partners LLC
Copyright (c) 2014-2015 Fraunhofer Fokus
Copyright (c) 2014-2015 MITRE
Copyright (c) 2014-2015 Otto-von-Guericke University of Magdeburg
Copyright (c) 2014-2015 Athan Services"@en,
	rdfs:label "Distributed Ontology, Model, and Specification Language (DOL) Terminology Ontology"@en,
        sm:isNormative "true"^^xsd:boolean,
    sm:contentLanguage "http://www.omg.org/spec/ODM/"^^xsd:anyURI,
    sm:fileAbstract "This ontology covers the terminology of the Distributed Ontology, Model, and Specification Language (DOL) and is a normative part of its specification."@en,
    sm:filename "dol-ontology.omn",
    dct:license "http://www.omg.org/techprocess/ab/SpecificationMetadata/MITLicense"^^xsd:anyURI,
    sm:contentLanguage "http://www.w3.org/standards/techs/owl#w3c_all"^^xsd:anyURI

AnnotationProperty: sm:copyright
AnnotationProperty: sm:isNormative
AnnotationProperty: sm:contentLanguage
AnnotationProperty: sm:fileAbstract
AnnotationProperty: sm:filename
AnnotationProperty: sm:license
AnnotationProperty: sm:contentLanguage

AnnotationProperty: dct:license

# AnnotationProperty: omv:hasFormalityLevel
# AnnotationProperty: omv:conformsToKnowledgeRepresentationParadigm
# AnnotationProperty: omv:isOfType
AnnotationProperty: dct:creator
	
AnnotationProperty: rdfs:label
AnnotationProperty: rdfs:seeAlso
AnnotationProperty: rdfs:comment
AnnotationProperty: rdfs:seeAlso
AnnotationProperty: owl:versionInfo
AnnotationProperty: owl:sameAs
	

AnnotationProperty: strictlyStrongerThan
    
AnnotationProperty: propagatesToAdjoint

    Annotations: 
        rdfs:comment "The subject class denotes a kind of mapping that, if it holds for a translation, also holds for the adjoint reduction."@en,
        rdfs:comment "Developers' note: This is just for informative purposes: Even though it probably does not go beyond OWL, it doesn't work for annotation properties in Protégé
Domain: owl:Class
Range: xsd:boolean"@en
    
    

    

    
AnnotationProperty: supportsSymbolKind

    Annotations: 
        rdfs:comment "Developers' note: This is just for informative purposes: Even though it probably does not go beyond OWL, it doesn't work for annotation properties in Protégé
Domain: OMSLanguage
Range: owl:Class that rdfs:subClassOf value NonLogicalSymbol"@en
    
    
AnnotationProperty: symbolKindIn
    
    Annotations: 
        rdfs:comment "Developers' note: This is just for informative purposes: It doesn't work for annotation properties
InverseOf: supportsSymbolKind"@en
    
    
AnnotationProperty: reifiedBy
    
    Annotations: 
        rdfs:comment "The subject property is reified by the object class."@en,
        rdfs:comment "Developers' note: This is just for informative purposes: It doesn't work for annotation properties
InverseOf: reifies"@en
    
    

    
AnnotationProperty: reifies

    Annotations: 
        rdfs:comment "The subject class reifies the object property."@en,
        rdfs:comment "Developers' note: This is just for informative purposes: Even though it probably does not go beyond OWL, it doesn't work for annotation properties in Protégé
Domain: owl:Class
Range: owl:ObjectProperty"@en
    
    

    
Datatype: xsd:string


    
ObjectProperty: isEmbeddableInto

    Annotations: 
	rdfs:label "is embeddable into"@en,
        rdfs:comment "The subject is embeddable into the object logic."@en
    
    SubPropertyOf: 
        isTranslatableTo,
        isExactlyMappableTo,
        isMappableToBijectivelyOnModels,
        isMappableToLogic
    
    Characteristics: 
        Transitive
    
ObjectProperty: isOmsIn
    Annotations: 
	rdfs:label "is OMS in"@en,
        rdfs:comment "The subject is an OMS participating in a DOL library, which is the object."@en

    InverseOf: 
        hasOMS
    SubPropertyOf: isLinguisticallyRelatedTo

    
ObjectProperty: isTranslatableFrom

    Annotations: 
	rdfs:label "is translatable from"@en,
        rdfs:comment "There is a translation from the object to the subject."@en
    
    SubPropertyOf: 
        isMappableFrom
    
    InverseOf: 
        isTranslatableTo
    
    
ObjectProperty: hasSequenceMember
	
    Annotations: 
	rdfs:label "has sequence member"@en,
        skos:definition "The inverse of the sequence membership relation."@en,
        skos:note "this is a lingustic property, because it is about sequences of linguistic entities that occur in a text."@en

    InverseOf: 
        isMemberOf
    SubPropertyOf: isLinguisticallyRelatedTo
	
ObjectProperty: hasMember
	
    Annotations: 
	rdfs:label "has member"@en,
        skos:definition "The inverse of the set membership relation."@en

    Domain: 
        Set
    Range: 
        MathematicalEntity
    
    InverseOf: 
        isMemberOf
    SubPropertyOf: isMathematicallyRelatedTo
    
    
ObjectProperty: isFaithfullyMappableTo

    Annotations: 
	rdfs:label "is faithfully mappable to"@en,
        rdfs:comment "There is a faithful mapping from the subject to the object logic."@en
    
    SubPropertyOf: 
        isMappableToLogic
    
    Characteristics: 
        Transitive
    SubPropertyOf: isMathematicallyRelatedTo
    
    
ObjectProperty: isMappableToLogic

    Annotations: 
	rdfs:label "is mappable to logic"@en,
        rdfs:comment "There is a mapping from the subject logic to the object logic."@en
    
    SubPropertyOf: 
        isMappableTo
    
    Characteristics: 
        Transitive
    
    InverseOf: 
        isMappableFromLogic
    SubPropertyOf: isMathematicallyRelatedTo
        
ObjectProperty: isExtensionOf
	
   Annotations: 
        rdfs:comment "Relation between two OMS. The subject OMS is an extension of the object OMS, i.e. the sets of non-logical symbols and sentences of the subject OMS are supersets of those of the object OMS."@en
    Domain: 
        OMS
    
    Range: 
        OMS

    Annotations: 
        skos:altLabel "is extension of"@en,
        skos:prefLabel "extends"@en
    
    SubPropertyOf: 
        isLinguisticallyRelatedTo
    
    SubPropertyChain: 
        isMappedBy o extendsTo
    
    Characteristics: 
        Transitive
    
    Domain: 
        OMS
    
    Range: 
        OMS
    
    InverseOf: 
        isSubOMSOf
    
    
    
ObjectProperty: isWeaklyExactlyMappableTo

    Annotations: 
	rdfs:label "is weakly exactly mappable to"@en,
        rdfs:comment "There is a weakly exact mapping from the subject to the object logic."@en
    
    SubPropertyOf: 
        isMappableToLogic
    
    Characteristics: 
        Transitive
    
    
ObjectProperty: isSubLanguageOf

    Annotations: 
        rdfs:comment "The subject is a sublanguage of the object language.  Supported logics are shared along the inverse of this property."@en,
        skos:definition "syntactically specified subset of a given language, consisting of a subset of its terminal and nonterminal symbols and grammar rules"@en,
        rdfs:label "is sublanguage of"@en
        
    SubPropertyOf: 
        isTranslatableTo,
        isMappableToLanguage, isLinguisticallyRelatedTo

    Characteristics: 
        Transitive
    
    Domain: 
        Language
    
    Range: 
        Language
    
    
ObjectProperty: specifiesSemanticsOf
    Annotations: 
	rdfs:label "specifies semantics of"@en,
        rdfs:comment "The semantics of [a subset of] the object language can be specified in terms of the subject logic."@en

    InverseOf: 
        supportsLogic
    SubPropertyOf: isSemanticallyRelatedTo
    
    
ObjectProperty: isTranslatableTo

    Annotations: 
	rdfs:label "is translatable to"@en,
        rdfs:comment "There is a translation from the subject to the object."@en
    
    SubPropertyOf: 
        isMappableTo
    
    Characteristics: 
        Transitive
    
    InverseOf: 
        isTranslatableFrom
    
    
ObjectProperty: mapsFrom

    Annotations: 
        rdfs:comment "The subject mapping maps from the object into something of the same type as the object."@en,
        rdfs:comment "Developers' note: enforcing the constraint that a mapping must map into something of the same type goes beyond OWL."@en
    
    Characteristics: 
        Functional
    
    Domain: 
        Mapping
    
    InverseOf: 
        isSourceOfMapping
    
    Annotations: 
        skos:definition "relationship between a mapping and its domain"@en,
        rdfs:label "maps from"@en
    
    Characteristics: 
        Functional
    
    Domain: 
        Mapping
    
    InverseOf: 
        isMappedBy
	
    SubPropertyOf: isRelatedAsPartOfMapsTo	
    
ObjectProperty: isExactlyMappableTo

    Annotations: 
	rdfs:label "is exactly mappable to"@en,
        rdfs:comment "There is an exact mapping from the subject to the object logic."@en
    
    SubPropertyOf: 
        isWeaklyExactlyMappableTo
    
    Characteristics: 
        Transitive
    SubPropertyOf: isMathematicallyRelatedTo
    
    
ObjectProperty: isLanguageOf

    Annotations: 
	rdfs:label "is language of"@en,
        rdfs:comment "Developers' note: The reasoners in Protégé don't like us to say the following.  Together with the SubPropertyChain specified for supportsSerialization it would go beyond OWL DL anyway.
SubPropertyChain: serialization o serializes"@en,
        skos:definition "the language of an OMS"@en
    
    Characteristics: 
        Functional
    
    Domain: 
        OMS
    
    Range: 
        OMSLanguage
    SubPropertyOf: isLinguisticallyRelatedTo
    
    
ObjectProperty: isMappableToBijectivelyOnModels

    Annotations: 
	rdfs:label "is mappable to bijectively on models"@en,
        rdfs:comment "There is a model-bijective mapping from the subject to the object logic."@en
    
    SubPropertyOf: 
        isModelExpansivelyMappableTo,
        isWeaklyExactlyMappableTo
    
    Characteristics: 
        Transitive
    
    
ObjectProperty: isMappingIn
    Annotations: 
	rdfs:label "is mapping in"@en,
        rdfs:comment "The object is a DOL library, in which the subject is a mapping between two participating OMS."@en

    InverseOf: 
        hasMapping
    SubPropertyOf: isLinguisticallyRelatedTo
    
    
ObjectProperty: hasOMS

    Annotations: 
	rdfs:label "has OMS"@en,
        rdfs:comment "The subject is a DOL library, in which the object is a participating heterogeneous OMS."@en
    
    SubPropertyOf: 
        hasMember
    
    Range: 
        OMS
    
    InverseOf: 
        isOmsIn
    SubPropertyOf: isLinguisticallyRelatedTo
    
    
ObjectProperty: isReducibleTo

    Annotations: 
	rdfs:label "is reducible to"@en,
        rdfs:comment "There is a reduction from the subject to the object."@en
    
    SubPropertyOf: 
        isMappableTo
    
    Characteristics: 
        Transitive
    
    InverseOf: 
        isReducibleFrom
    SubPropertyOf: isMathematicallyRelatedTo
    
    
ObjectProperty: hasTarget

    Annotations: 
	rdfs:label "has target"@en,
        skos:definition "the target OMS of a mapping"@en
    
    Characteristics: 
        Functional
    
    Domain: 
        OMSMapping
    
    Range: 
        OMS
    SubPropertyOf: isLinguisticallyRelatedTo
    
    
ObjectProperty: hasSource

    Annotations: 
	rdfs:label "has source"@en,
        skos:definition "the source OMS of a mapping"@en
    
    Characteristics: 
        Functional
    
    Domain: 
        OMSMapping
    
    Range: 
        OMS
    SubPropertyOf: isLinguisticallyRelatedTo
    
    
ObjectProperty: hasExactLogicalExpressivity

    Annotations: 
	rdfs:label "has exact logical expressivity"@en,
        rdfs:comment "The subject language has exactly the expressivity of the object logic."@en
    
    SubPropertyOf: 
        supportsLogic
    SubPropertyOf: isSemanticallyRelatedTo
    
    
ObjectProperty: serializes
    Annotations: 
        rdfs:comment "The subject is a serialization for the object language. For example, Manchester syntax serializes OWL"@en

    InverseOf: 
        supportsSerialization

    Annotations: 
        rdfs:label "serializes"@en
    
    Domain: 
        Serialization
    
    Range: 
        OMSLanguage
    SubPropertyOf: isLinguisticallyRelatedTo
    
    
    
ObjectProperty: isMonomorphicExtensionOf

    Annotations: 
	rdfs:label "is monomorphic extension of"@en,
        rdfs:comment "The subject OMS is a monomorphic extension of the object OMS. A monomorphic extension is an extension whose newly introduced non-logical symbols are interpreted in a way unique up to isomorphism."@en,
        strictlyStrongerThan isModelTheoreticallyConservativeExtensionOf
    
    SubPropertyOf: 
        isModelTheoreticallyConservativeExtensionOf
    
    
ObjectProperty: hasInterpretation

    Annotations: 
	rdfs:label "has interpretation"@en,
        rdfs:comment "The subject is a DOL library, in which the object is an interpretation between two participating OMS."@en
    
    SubPropertyOf: 
        hasMapping
    
    Range: 
        Interpretation
    
    InverseOf: 
        isInterpretationIn
    SubPropertyOf: isLinguisticallyRelatedTo
    
    
ObjectProperty: hasAlignment

    Annotations: 
	rdfs:label "has alignment"@en,
        rdfs:comment "The subject is a DOL library, in which the object is an alignment between two participating OMS."@en
    
    SubPropertyOf: 
        hasMapping
    
    Range: 
        Alignment
    
    InverseOf: 
        isAlignmentIn
    SubPropertyOf: isLinguisticallyRelatedTo
    
    
ObjectProperty: isSequenceMemberOf
    Annotations: 
	rdfs:label "is sequence memberOf"@en,
        skos:definition "The sequence membership relation."@en

    InverseOf: 
        hasSequenceMember
    SubPropertyOf: isLinguisticallyRelatedTo
    
ObjectProperty: isMemberOf
    Annotations: 
	rdfs:label "is member of"@en,
        skos:definition "The set membership relation."@en

    InverseOf: 
        hasMember
    SubPropertyOf: isMathematicallyRelatedTo
    Domain: MathematicalEntity
    Range: Set	
	
    
ObjectProperty: isModelTheoreticallyConservativeExtensionOf

    Annotations: 
	rdfs:label "is model theoretically conservative extension of"@en,
        rdfs:comment "The subject OMS is a model-theoretic conservative extension of the object OMS. A model-theoretic conservative extension is an extension that does not lead to a restriction of class of models of an OMS."@en,
        strictlyStrongerThan isConsequenceTheoreticallyConservativeExtensionOf
    
    SubPropertyOf: 
        isConservativeExtensionOf
    
ObjectProperty: supportsLogic

    Annotations: 
	rdfs:label "supportsL lgic"@en,
        rdfs:comment "The semantics of [a subset of] the subject language can be specified in terms of the object logic."@en
	
    SubPropertyOf: isSemanticallyRelatedTo
    
    SubPropertyChain: 
        inverse (isSubLanguageOf) o supportsLogic,
        supportsLogic o  inverse (isSubLogicOf)
    
    Domain: 
        OMSLanguage
    
    Range: 
        Logic
    
    InverseOf: 
        specifiesSemanticsOf

    Annotations: 
        rdfs:label "supports logic"@en,
        skos:definition "logic represented by a satisfaction relation of the language."@en
    
    Domain: 
        OMSLanguage
    
    Range: 
        Logic
    
ObjectProperty: isMappableToLanguage

    Annotations: 
	rdfs:label "is mappable to language"@en,
        rdfs:comment "There is a mapping from the subject language to the object language."@en
    
    SubPropertyOf: 
        isMappableTo, isLinguisticallyRelatedTo
    
    Characteristics: 
        Transitive
    
    InverseOf: 
        isMappableFromLanguage
    SubPropertyOf: isRelatedAsPartOfMapsTo	
    
    
ObjectProperty: isAlignmentIn
    Annotations: 
	rdfs:label "is alignment in"@en,
        rdfs:comment "The obbject is a DOL library, in which the subject is an alignment between two participating OMS."@en

    InverseOf: 
        hasAlignment
    SubPropertyOf: isLinguisticallyRelatedTo
    
    
ObjectProperty: isSourceOfMapping
   Annotations: 
	rdfs:label "is source of mapping"@en,
        rdfs:comment "The object mapping maps from the subject into something of the same type as the subject."@en
    InverseOf: 
        mapsFrom
    
    SubPropertyOf: isRelatedAsPartOfMapsTo	
    
ObjectProperty: mapsTo

    Annotations: 
        rdfs:comment "The subject mapping maps from something into the object (which is of the same type).  Enforcing the latter constraint goes beyond OWL."@en
    
    Characteristics: 
        Functional
    
    Domain: 
        Mapping

    Annotations: 
        skos:definition "relationship between a mapping and its codomain"@en,
        rdfs:label "maps to"@en
    
    Characteristics: 
        Functional
    
    Domain: 
        Mapping
    
    SubPropertyOf: isRelatedAsPartOfMapsTo	
    
    
ObjectProperty: isSubLogicOf

    Annotations: 
        rdfs:comment "The subject is a sublogic of the object."@en
    
    SubPropertyOf: 
        isEmbeddableInto
    
    SubPropertyOf: isMathematicallyRelatedTo
    SubPropertyChain: 
         inverse (hasExactLogicalExpressivity) o isSubLanguageOf o hasExactLogicalExpressivity
    
    Annotations: 
        skos:definition "a logic that is a syntactic restriction of another logic, inheriting its semantics"@en,
        rdfs:label "is sublogic of"@en
    
    Characteristics: 
        Transitive
    
    Domain: 
        Logic
    
    Range: 
        Logic
    
    
ObjectProperty: isInterpretationIn
    Annotations: 
	rdfs:label "is interpretation in"@en,
        rdfs:comment "The object is a DOL library, in which the subject is an interpretation between two participating OMS."@en

    InverseOf: 
        hasInterpretation
    SubPropertyOf: isLinguisticallyRelatedTo
    
    
ObjectProperty: isMappableFrom

    Annotations: 
	rdfs:label "is mappable from"@en,
        rdfs:comment "There is a mapping from the object to the subject."@en
    
    InverseOf: 
        isMappableTo
	
    SubPropertyOf: isRelatedAsPartOfMapsTo	
    
    
ObjectProperty: isCompositionOf

    Annotations: 
	rdfs:label "is composition of"@en,
        rdfs:comment "Range can't be specified in OWL DL"@en,
        rdfs:comment "Developers' note: The subject mapping is the composition of the object list of mappings (list item 1 ∘ list item 2 ∘ … ∘ list item n).  All elements of the latter list must be instances of the same class as the subject.  (Enforcing the latter constraint goes beyond OWL.)"@en
    
    SubPropertyOf: isMathematicallyRelatedTo
    
    
ObjectProperty: isSimplyTheoroidallyMappableTo

    Annotations: 
	rdfs:label "is simply theoroidally mappable to"@en,
        rdfs:comment "There is a simple theoroidal mapping from the subject to the object logic."@en
    
    SubPropertyOf: 
        isMappableToLogic
    SubPropertyOf: isMathematicallyRelatedTo
    
    Characteristics: 
        Transitive
    
    
ObjectProperty: hasLogic

    Annotations: 
	rdfs:label "has logic"@en,
        rdfs:comment "the logic in which an OMS is formalized"@en,
        skos:definition "specification of valid reasoning that comprises signatures (user defined vocabularies), models (interpretations of these), sentences (constraints on models), and a satisfaction relation between models and sentences."@en,
        rdfs:comment "Developers' note: The reasoners in Protégé don't like us to say the following, which makes hasLogic a non-simple property.  hasLogic is not used in cardinality restrictions, so it _should_ be OK to say the following, but in practice it doesn't work.
SubPropertyChain: semanticallyDenotes o hasLogic"@en
    Characteristics: 
        Functional
    
    Domain: 
        OMS or OMSSemanticObject
    
    Range: 
        Logic
    
    SubPropertyOf: isSemanticallyRelatedTo
    
ObjectProperty: isModelExpansivelyMappableTo

    Annotations: 
	rdfs:label "is model expansively mappable to"@en,
        rdfs:comment "There is a model-expansive mapping from the subject to the object logic."@en
    
    SubPropertyOf: 
        isFaithfullyMappableTo
    
    Characteristics: 
        Transitive
    
    
ObjectProperty: isMappableFromLogic

    Annotations: 
	rdfs:label "mappable from logic"@en,
        rdfs:comment "There is a mapping from the object logic to the subject logic."@en
    
    InverseOf: 
        isMappableToLogic
    SubPropertyOf: isMathematicallyRelatedTo
    
    
ObjectProperty: isConsequenceTheoreticallyConservativeExtensionOf
    Annotations: 
	rdfs:label "is consequence theoretically conservative extension of"@en,
        rdfs:comment "The subject OMS is a consequence-theoretic conservative extension of the object OMS. A consequence-theoretic conservative extension is an extension that does not add new theorems (in terms of the unextended signature)."@en
    SubPropertyOf: 
        isConservativeExtensionOf
    
ObjectProperty: isProfileOf
    Annotations: 
        rdfs:comment "The subject is a isProfile of the object language.  This is a stronger notion than just being a sublanguage.  Supported serializations are shared along this property."@en,
        rdfs:label "is profile of"@en,
        skos:definition "see Class 'profile'"@en
    
    SubPropertyOf: 
        isSubLanguageOf, isLinguisticallyRelatedTo
    
    Domain: 
        Profile
    
    Range: 
        OMSLanguage
    

ObjectProperty: isMappableFromLanguage

    Annotations: 
	rdfs:label "mappable from language"@en,
        rdfs:comment "There is a mapping from the object language to the subject language."@en
    
    InverseOf: 
        isMappableToLanguage
    SubPropertyOf: isLinguisticallyRelatedTo, isRelatedAsPartOfMapsTo	
    
    
ObjectProperty: isSerializedIn

    Annotations: 
	rdfs:label "is serialized in"@en,
        rdfs:comment "the textual syntax in which an OMS is written"@en
    
    Characteristics: 
        Functional
    
    Domain: 
        OMS
    
    Range: 
        Serialization
    
    SubPropertyOf: isLinguisticallyRelatedTo
    
ObjectProperty: isMappableTo

    Annotations: 
	rdfs:label "is mappable to"@en,
        rdfs:comment "There is a mapping from the subject to the object."@en
    
    SubPropertyChain: 
        isSourceOfMapping o mapsTo
    
    Characteristics: 
        Transitive
    
    InverseOf: 
        isMappableFrom
    
    SubPropertyOf: isRelatedAsPartOfMapsTo	
    
ObjectProperty: hasMapping

    Annotations: 
	rdfs:label "has mapping"@en,
        rdfs:comment "The subject is a DOL library, in which the object is a mapping between two participating OMS."@en
    
    SubPropertyOf: 
        hasMember, isLinguisticallyRelatedTo
    
    Range: 
        OMSMapping
    
    InverseOf: 
        isMappingIn
    
ObjectProperty: isWeakDefinitionalExtensionOf
    Annotations: 
	rdfs:label "is weak definitional extension of"@en,
        rdfs:comment "The subject OMS is a weak definitional extension of the object OMS. A weak definitional extension is an extension whose newly introduced
   non-logical symbols can be interpreted in at most one way."    
    SubPropertyOf: isMathematicallyRelatedTo
    
    
    
ObjectProperty: isPlainlyMappableTo

    Annotations: 
	rdfs:label "is plainly mappable to"@en,
        rdfs:comment "There is a plain mapping from the subject to the object logic."@en
    
    SubPropertyOf: 
        isSimplyTheoroidallyMappableTo
    
    Characteristics: 
        Transitive
    
    
ObjectProperty: supportsSerialization

    Annotations: 
	rdfs:label "supports serialization"@en,
        rdfs:comment "Developers' note: The reasoners in Protégé don't like us to say the following.  Together with the SubPropertyChain specified for language it would go beyond OWL DL anyway.
SubPropertyChain: isProfileOf o supportsSerialization"@en,
        rdfs:comment "Note that the serialization should be as specific as possible, i.e. one should not say that ``OWL can be serialized in XML'' and ``Common Logic can be serialized in XML'', but instead ``OWL can be serialized in OWL XML'' and ``Common Logic can be serialized in XCL'', taking into account that OWL XML and XCL are two different XML languages."@en,
        rdfs:comment "OMS in the subject language can be serialized in the object serialization."@en
    
    Characteristics: 
        InverseFunctional
    
    Domain: 
        OMSLanguage
    
    Range: 
        Serialization
    
    InverseOf: 
        serializes
    SubPropertyOf: isLinguisticallyRelatedTo
    
    
ObjectProperty: isReducibleFrom

    Annotations: 
	rdfs:label "is reducible from"@en,
        rdfs:comment "There is a reduction from the object to the subject."@en
    
    SubPropertyOf: 
        isMappableFrom
    
    InverseOf: 
        isReducibleTo
    
    
DataProperty: mediaType

    Annotations: 
        rdfs:comment "the media type (MIME type) of a serialization"@en
    
    Characteristics: 
        Functional
    
    Domain: 
        Serialization
    
    Range: 
        xsd:string
    
    
DataProperty: prefFilenameExtension

    Annotations: 
        skos:definition "the preferred filename extension for a serialization"@en
    
    Characteristics: 
        Functional
    
    Domain: 
        Serialization
    
    Range: 
        xsd:string
    
    
DataProperty: altFilenameExtension

    Annotations: 
        skos:definition "an alternative filename extension for a serialization"@en
    
    Domain: 
        Serialization
    
    Range: 
        xsd:string
    
    

    
Class: WeaklyExactMapping

    Annotations: 
	rdfs:label "weakly exact mapping"@en,
        skos:definition "logic mapping that is weakly compatible with certain DOL structuring constructs"@en,
        propagatesToAdjoint "true"^^xsd:boolean,
        reifies isWeaklyExactlyMappableTo
    
    SubClassOf: 
        LogicMapping
    
    
Class: ExactMapping

    Annotations: 
	rdfs:label "exact mapping"@en,
        skos:definition "logic mapping that is compatible with certain DOL structuring constructs"@en,
        propagatesToAdjoint "true"^^xsd:boolean,
        reifies isExactlyMappableTo
    
    SubClassOf: 
        WeaklyExactMapping
    
    
Class: DOLLibrary

    Annotations: 
	rdfs:label "DOL library"@en,
        skos:definition "collection of named OMS and OMS networks, possibly written in different OMS languages, linked by named OMS mappings."@en,    
        skos:note "collection is used here in the sense of syntactic collection"@en
    SubClassOf: DOLEntity, semanticallyDenotes some GlobalEnvironment


    
Class: ModelExpansiveMapping

    Annotations: 
	rdfs:label "model expansive mapping"@en,
        skos:definition "logic mapping that has a surjective model translation (ensuring faithfulness of the mapping)"@en,
        propagatesToAdjoint "true"^^xsd:boolean,
        reifies isModelExpansivelyMappableTo
    
    SubClassOf: 
        FaithfulMapping
    
    
	
    
    
Class: SubLogic

    Annotations: 
	rdfs:label "sublogic"@en,
        rdfs:comment "logic embedding that is 'syntactic' in the sense that signature and sentence translations are inclusions."@en,
        reifies isSubLogicOf
    
    SubClassOf: 
        Embedding
    
    
Class: Sentence
    Annotations: 
        rdfs:comment "a sentence in an OMS"@en,
        skos:note "It is quite common that sentences are required to be closed (i.e.\\ have no free variables). However, this depends on the OMS language at hand."@en,
        skos:note "In a model, on the one hand, a sentence is always true or false. In an OMS, on the other hand, a sentence can have several logical statuses: it can be an axiom, if postulated to be true; a theorem, if proven from other axioms and theorems; a conjecture, if expecting to be proven from other axioms and theorems; or have another of many possible statuses."@en,
        skos:note "A sentence can conform to one or more signatures (namely those signatures containing all non-logical symbols used in the sentence)."@en,
        skos:definition "term that is either true or false in a given model, i.e.\\ which is assigned a truth value in this model."@en,
        rdfs:label "sentence"@en
    
    SubClassOf: 
        Term
    

    
Class: View

    Annotations: 
        rdfs:comment "a view (also called interpretation) between two heterogeneous OMS in a DOL library"@en
    
    EquivalentTo: 
        Interpretation
    
    SubClassOf: 
        OMSMapping
    
    Annotations: 
        skos:note "An interpretation typically leads to proof obligations, \\ie one has to prove that axioms of the source OMS of the mapping are theorems in the target OMS."@en,
        skos:definition "OMS mapping that postulates a relation between two OMS"@en,
        skos:altLabel "interpretation"@en,
        rdfs:label "view"@en,
        skos:note " When an interpretation is given as a set of correspondences, these are given as tuples, where the type of relationship is given by the specific kind of interpretation. "@en
    
    SubClassOf: 
        OMSMapping
    
    
Class: Embedding

    Annotations: 
	rdfs:label "embedding"@en,
        skos:definition "logic mapping that embeds the source into the target logic, using components that are embeddings and (in the case of model translations) isomorphism"@en,
        reifies isEmbeddableInto
    
    SubClassOf: 
        ExactMapping,
        LogicMapping,
        LogicTranslation,
        ModelBijectiveMapping
    
Class: OMS

    Annotations: 
        skos:definition "a basic or structured ontology, specification or MDE model"@en,
        rdfs:label "OMS (ontology, specification or MDE model)"@en,
        skos:note "An OMS is a collection of expressions (like non-logical symbols, sentences and structuring elements) in a given OMS language (or several such languages)"@en,
        skos:note "An OMS can be written in different OMS language serializations."@en,
        skos:note "collection is used here in the sense of syntactic collection"@en,
        skos:note "An OMS has a single signature and model class over that signature as its model-theoretic semantics."@en

    
    EquivalentTo: 
        HeterogeneousOMS
         or HomogeneousOMS,
        ElusiveOMS
         or FlattenableOMS
    
    SubClassOf: 
        usesLanguage some OMSLanguage, 
 	semanticallyDenotes some OMSSemanticObject,
	hasLogic some Logic,
        hasSignature some Signature, 
	hasSentences some SetOfSentences, hasModels some ClassOfModels
    SubClassOf: DOLEntity
    
    
Class: Ontology

    Annotations: 
	rdfs:label "ontology"@en,
        skos:definition "logical theory that is used as a shard conceptualization"@en

    SubClassOf:
        OMS
    
Class: MDEModel

    Annotations: 
	rdfs:label "MDE model"@en,
        skos:definition "logical theory that is used as a model in the sense of model-driven engineering (MDE)"@en,
    	skos:note "Not to be confused with the term \termref{model} in the sense
of logic (model theory)."@en
    SubClassOf:
        OMS

    
Class: Specification

    Annotations: 
	rdfs:label "specification"@en,
        skos:definition "logical theory that is used as a formal specification"@en

    SubClassOf:
        OMS
    
Class: Interpretation
    Annotations: 
	rdfs:label "interpretation"@en,
	skos:altLabel "view"@en,
	skos:altLabel "refinement"@en,
        skos:definition "OMS mapping that postulates a specialization relation between two OMS along a morphism between their signatures"@en

    EquivalentTo: 
        View
	    
    SubClassOf: 
        OMSMapping
   
    
Class: OMSLanguageTranslation

    Annotations: 
        skos:definition "a mapping (translation or reduction) between two OMS languages"@en,
        propagatesToAdjoint "true"^^xsd:boolean
    
    SubClassOf: 
        Mapping, 
        (mapsFrom exactly 1 OMSLanguage)
         and (mapsTo exactly 1 OMSLanguage)

    Annotations: 
        rdfs:label "OMS language translation"@en,
        skos:note " An OMS language translation shall satisfy the property that the result of a translation is a well-formed text in the target language. "@en,
        skos:definition "mapping from constructs in the source OMS language to their equivalents in the target OMS language"@en
    
    SubClassOf: 
        LanguageMapping,
        mapsFrom exactly 1 OMSLanguage,
        mapsTo exactly 1 OMSLanguage

Class: Logic
    Annotations: 
        rdfs:label "logic"@en,
	rdfs:comment "a logic that defines the semantics of an language"@en,
        skos:example " $\\mathcal{SROIQ}(D)$ is the logic underlying OWL 2 DL. "@en,
        skos:note " Most OMS languages have an underlying logic. "@en,
        rdfs:label "logic"@en,
        skos:definition "specification of valid reasoning that comprises signatures, sentences, models, and a satisfaction relation between models and sentences"@en,
        skos:note " See annex~\\ref{a:rdf-logic-vocab} for the organization of the relation between OMS languages and their logics and serializations. "@en
    
    SubClassOf: 
        isFormalizedBy some Institution
    SubClassOf: MathematicalEntity

    
Class: SimpleTheoroidalMapping

    Annotations: 
	rdfs:label "simple theoroidal mapping"@en,
	skos:definition "logic mapping that maps signatures to theories"@en,
	rdfs:comment "the resulting theory tpyically contains infrastructure axioms that are needed for expressing the logic mapping"@en,
        propagatesToAdjoint "true"^^xsd:boolean,
        reifies isSimplyTheoroidallyMappableTo,
        rdfs:comment "orthogonal to WeaklyExactMapping and FaithfulMapping"@en
    
    EquivalentTo: 
        LogicMapping
         and (not (PlainMapping))
    
    SubClassOf: 
        LogicMapping
    
    DisjointWith: 
        PlainMapping,
        
            Annotations: rdfs:comment "Developers' note: Protégé 4.2 doesn't like 'Class: OMSMapping DisjointUnionOf: PlainMapping, SimpleTheoroidalMapping', so we do it this way:"@en
        PlainMapping
   

Class: LogicMapping

    Annotations: 
        rdfs:comment "a mapping (translation or reduction) between two logics"@en,
        propagatesToAdjoint "true"^^xsd:boolean
    
    SubClassOf: 
        Mapping,
        (mapsFrom exactly 1 Logic)
         and (mapsTo exactly 1 Logic)

    Annotations: 
        rdfs:label "logic mapping"@en,
        skos:definition "mapping between logics"@en
    
    EquivalentTo: 
        (mapsFrom exactly 1 Logic)
         and (mapsTo exactly 1 Logic)
    
    SubClassOf: 
        Mapping
    
    
Class: Refinement
    Annotations: 
	skos:definition "OMS mapping that postulates a specialization relation between two OMS along a morphism between their signatures"@en,
        rdfs:comment "refinement"@en,
        rdfs:label "refinement"@en

    
    SubClassOf: 
        OMSMapping
    
    
Class: OMSReduction

    Annotations: 
	rdfs:label "OMS reduction"@en,
        reifies isReducibleTo,
        skos:definition "DOL structured OMS expressing the restriction of an OMS to a smaller signature."@en
    
    SubClassOf: 
        DOLStructuredOMS
    
    DisjointWith: 
        OMSTranslation
	    
    SubClassOf: 
        OMSMapping, hasPart some DOLStructuredOMS
    

Class: BasicOMS
    Annotations: 
        rdfs:comment "a basic OMS (in a single language, logic, and serialization)"@en,
        rdfs:label "basic OMS"@en,
        skos:definition "unstructured native OMS that may be used as a building block for a larger OMS, denoting a logical theory"@en
    
    SubClassOf: 
        NativeOMS
    
    SubClassOf: 
        hasPart exactly 1 OMSDocumentation,
        FlattenableOMS,
        semanticallyDenotes some LogicalTheory
    

Class: FaithfulMapping

    Annotations: 
	rdfs:label "faithful mapping"@en,
        skos:definition "logic mapping that preserves and reflects logical consequence"@en,
        propagatesToAdjoint "true"^^xsd:boolean,
        reifies isFaithfullyMappableTo
    
    SubClassOf: 
        LogicMapping
    
	
Class: OMSMapping

    Annotations: 
        rdfs:comment "a mapping between two heterogeneous OMS in a DOL library"@en, 
        reifies isMappableTo,
        rdfs:label "OMS mapping"@en,
        skos:definition "relationship between two OMS, typically given as a set of correspondences"@en
    
    EquivalentTo: 
        (mapsFrom exactly 1 OMS)
         and (mapsTo exactly 1 OMS)
    
    SubClassOf: 
        DOLEntity
    
    
Class: DefaultMapping
    Annotations: 
	rdfs:label "default mapping"@en,
        skos:definition "logic mapping that will be chosen by default if only the source and target logic are given"@en,
        propagatesToAdjoint "true"^^xsd:boolean

    SubClassOf: 
        LogicMapping
    
    
Class: PlainMapping
    Annotations: 
	rdfs:label "plain mapping"@en,
        skos:definition "logic mapping that maps signatures to signatures and therefore does not use infrastructure axioms"@en,
        reifies isPlainlyMappableTo,
        propagatesToAdjoint "true"^^xsd:boolean
    
    SubClassOf: 
        LogicMapping
    
    DisjointWith: 
        SimpleTheoroidalMapping
        
            Annotations: rdfs:comment "Developers' note: Protégé 4.2 doesn't like 'Class: OMSMapping DisjointUnionOf: PlainMapping, SimpleTheoroidalMapping', so we do it this way:"@en
    
Class: Serialization
    Annotations: 
        rdfs:comment "a serialization of an language"@en,
        skos:definition "specific syntactic encoding of a given OMS language"@en,
        skos:example " Common Logic uses the term ``dialect''; the following are standard Common Logic dialects: Common Logic Interchange Format (CLIF), Conceptual Graph Interchange Format (GCIF), eXtended Common Logic Markup Language (XCL)."@en,
        rdfs:label "OMS serialization"@en,
        skos:note "Serializations serve as standard formats for exchanging OMS between tools."@en,
        skos:example "OWL uses the term ``serialization''; the following are standard OWL serializations: OWL functional-style syntax, OWL/XML, OWL Manchester syntax, plus any standard serialization of RDF (e.g.  RDF/XML, Turtle, \\dots). However, RDF/XML is the only one tools are required to implement. "@en,
        rdfs:comment "synonymous to 'concrete syntax'"@en
    
    SubClassOf: 
        serializes some OMSLanguage, LinguisticEntity
    

Class: OMSLanguage
    Annotations: 
        rdfs:comment "a language for OMS (ontologies, models or specifications)"@en
    
    SubClassOf: 
        (supportsLogic some Logic)
         and (supportsSerialization some Serialization)
         and (supportsLogic only Logic)
         and (supportsSerialization only Serialization)

    Annotations: 
        skos:definition "language equipped with a formal, declarative, logic-based semantics, plus non-logical annotations"@en,
        rdfs:label "OMS language"@en,
        skos:note " An OMS language is used for the formal specification of OMS."@en,
        skos:example " OMS languages include OWL, Common Logic, F-logic, UML class diagrams, RDFS, and OBO. "@en
    
    SubClassOf: 
        supportsLogic some Logic,
        Language

	
Class: Language
    Annotations: 
        skos:definition "collection of expressions"@en,
        skos:note "collection is used here in the sense of syntactic collection"@en,
        rdfs:label "language"@en
    
    SubClassOf: 
        hasPart some CollectionOfExpressions
    SubClassOf: LinguisticEntity
    

    
    
Class: ModelBijectiveMapping
    Annotations: 
	rdfs:label "model bijective mapping"@en,
        skos:definition "logic mapping that has a bijective mapping of models"@en,
        reifies isMappableToBijectivelyOnModels,
        propagatesToAdjoint "true"^^xsd:boolean
    
    SubClassOf: 
        WeaklyExactMapping,
        ModelExpansiveMapping
    
    
Class: Alignment

    Annotations: 
	rdfs:label "alignment"@en,
        skos:definition "an OMS mapping expressing a collection of relations between entities of the two OMS"@en,
        rdfs:comment "an alignment between two heterogeneous OMS in a DOL library"@en
    
    SubClassOf: 
        OMSMapping, hasPart some Correspondence
    
DisjointClasses: 
        Alignment,Interpretation

DisjointClasses:
        Logic,OMSMapping,OMS,OMSLanguage,Serialization

	
ObjectProperty: impliedExtendsTo

    Annotations: 
        skos:definition "the relation of a model-theoretic conservative extension that does not introduce new non-logical symbols"@en,
        rdfs:label "implied extends to"@en
    
    SubPropertyOf: 
        definitionallyExtendsTo
    
    Domain: 
        ImpliedExtensionMapping
    
ObjectProperty: isSubOMSOf

    Annotations: 
        rdfs:label "is subOMS of"@en,
        skos:definition "OMS whose sets of non-logical symbols and sentences are subsets of those present in a given larger OMS"@en
    
    Characteristics: 
        Transitive
    
    Domain: 
        OMS
    
    Range: 
        OMS
	
    SubPropertyOf: isLinguisticallyRelatedTo
	
ObjectProperty: isCombinationOf
	
    Annotations: 
        skos:example "Consider an ontology involving a concept Person, and another one involving Human being, and an alignment that relates these to concepts. In the combination of the ontologies along the alignment, there is only one concept, representing both Person and Human being."@en,
        rdfs:label "is combination of OMS"@en,
        skos:definition "aggregation of all the OMS in an OMS network, where non-logical symbols are shared according to the OMS mappings in the OMS network "@en
    
    Domain: 
        Combination
    
    Range: 
        OMSNetwork
    
    SubPropertyOf: isLinguisticallyRelatedTo
    
    
ObjectProperty: isAdjointOf

    Annotations: 
        rdfs:comment "The subject is a translation (or reduction) that shares its sentence and model translation with the object reduction (or translation). The signature translations are adjoint to each other (in the sense of category theory)."@en,
        rdfs:label "is adjoint of"@en
    
    Domain: 
        LogicTranslation
    
    Range: 
        LogicReduction
    SubPropertyOf: isMathematicallyRelatedTo
    
    
ObjectProperty: definitionallyExtendsTo
    Annotations: 
        rdfs:comment "the object is a definitional extension of the subject"@en,
        rdfs:label "definitionally extends to"@en
    
    SubPropertyOf: 
        conservativelyExtendsTo
    
    Domain: 
        DefinitionalExtensionMapping
    
    
ObjectProperty: isOMSUnionOf
    Annotations: 
        skos:definition "structured OMS expressing the combination of all constraints of a sequences of OMS"@en,
        rdfs:label "is union of OMS"@en
    
    Domain: 
        DOLStructuredOMS
    
    Range: 
        SequenceOfOMS
    
    SubPropertyOf: isLinguisticallyRelatedTo
    
ObjectProperty: isLogicallyInteroperableWith
    Annotations: 
        skos:definition "property of structured OMS, which may be written in different OMS languages supporting different logics, of being usable jointly in a coherent way (via suitable OMS language translations), such that the notions of their overall consistency and logical entailment have a precise logical semantics"@en,
        rdfs:label "is logically interoperable with"@en
    
    Characteristics: 
        Symmetric
    
    Domain: 
        StructuredOMS
    
    Range: 
        StructuredOMS
    
    SubPropertyOf: isLinguisticallyRelatedTo
    
ObjectProperty: isDefinitionalExtensionOf
    Annotations: 
        strictlyStrongerThan isMonomorphicExtensionOf,
        rdfs:comment "Developers' note: We need FOL, or the same reification approach as chosen for the different kinds of translations, for capturing that an extension is definitional if and only if it is weakly definitional and model-theoretically conservative."@en,
        skos:note " An extension $O_2$ of an OMS $O_1$ is a definitional extension, if each model of $O_1$ can be uniquely expanded to a model of $O_2$. "@en,
        skos:note " Each definitional extension is also a monomorphic extension but not vice versa. "@en,
        skos:definition "extension whose newly introduced non-logical symbols are interpreted in a unique way"@en,
        skos:note " $O_2$ being a definitional extension of $O_1$ implies a bijective correspondence between the classes of models of $O_2$ and $O_1$. "@en,
        rdfs:label "is definitional extension of"@en
    
    SubPropertyOf: 
        isMonomorphicExtensionOf, isWeakDefinitionalExtensionOf,         isModelTheoreticallyConservativeExtensionOf
    
    SubPropertyChain: 
        isMappedBy o definitionallyExtendsTo
    
    
ObjectProperty: isOMSDocumentationOf
    Annotations: 
        rdfs:label "is OMS documentation of"@en,
        skos:definition "relationship between an OMS documentation and the documented OMS"@en
        
#    InverseOf: 
#        documentsOMS
	
    Characteristics: 
        Functional
    
    Domain: 
        OMSDocumentation
    
    Range: 
        OMS
    
    SubPropertyOf: isLinguisticallyRelatedTo
    
ObjectProperty: isLanguageAspectOf
    Annotations: 
        skos:definition "a language asecpt is a set of language constructs of a given language, not necessarily forming a sublanguage"@en,
        rdfs:label "is language aspect of"@en
    
    InverseOf: 
        hasLanguageAspect
    SubPropertyOf: isLinguisticallyRelatedTo
    
    
ObjectProperty: formalizes
    Annotations: 
        rdfs:comment "The subject is a precise mathematical entity capturing the object (which is an informal or semi-formal entity)"@en,
        rdfs:label "formalizes"@en
    
    InverseOf: 
        isFormalizedBy
    SubPropertyOf: isSemanticallyRelatedTo
    
    
    
    
ObjectProperty: conservativelyExtendsTo
    Annotations: 
        rdfs:comment "The object is a conservative extension of the subject"@en,
        rdfs:label "conservatively extends to"@en
    
    SubPropertyOf: extendsTo, isLogicallyRelatedTo
    
    Domain: 
        ConservativeExtensionMapping
    
    
ObjectProperty: usesLanguage
    Annotations: 
        skos:definition "relation between something and a language used by one or more components of it."@en,
        rdfs:label "uses language"@en
    SubPropertyOf: isLinguisticallyRelatedTo
    
    
ObjectProperty: isElementOf
    Annotations: 
        skos:definition "any resource in an OMS (e.g. a non-logical symbol, a sentence, a correspondence, the OMS itself, ...) or a named set of such resources."@en,
        rdfs:label "is element of OMS"@en
    
    SubPropertyOf: 
        hasPart, isLinguisticallyRelatedTo
    
    Range: 
        OMS
    
    
    
ObjectProperty: isModelOfOMS
    Annotations: 
        rdfs:label "is a model of the OMS"@en,
        skos:definition "relationship between a model and an OMS where the model is a member of the model class of the OMS (which for flattenable OMS is equivalent to being a model of the signature of the OMS and satisfying all sentences in the OMS)."@en
    
    Domain: 
        Model
    
    Range: 
        OMS
    SubPropertyOf: isSemanticallyRelatedTo
    
    
ObjectProperty: hasHeterogeneousEnvironment
    Annotations: 
        skos:definition "relationship between the subject and a heterogeneous environment in which it is embedded or is associated with."@en,
        rdfs:label "has heterogeneous environment"@en
    
    Range: 
        HeterogeneousEnvironment
    SubPropertyOf: isMathematicallyRelatedTo
    
    
    
ObjectProperty: isConservativeExtensionOf
    Annotations: 
        rdfs:comment "the subject is a conservative extension of the object"@en,
        rdfs:label "is conservative extension of"@en
    
    SubPropertyOf: 
        isExtensionOf
    SubPropertyOf: isLogicallyRelatedTo
    
    SubPropertyChain: 
        isMappedBy o conservativelyExtendsTo
    
    InverseOf: 
        isModuleOf
    
    
    
ObjectProperty: hasLanguageAspect
    Annotations: 
        rdfs:label "has language aspect"@en,
        skos:definition "the relation between an OMS language and its language aspects"@en
    
    Domain: 
        OMSLanguage
    
    Range: 
        LanguageAspect
    
    InverseOf: 
        isLanguageAspectOf
    SubPropertyOf: isLinguisticallyRelatedTo
    
    
ObjectProperty: isModelOfSignature
    Annotations: 
        rdfs:label "is a model of the signature"@en,
        skos:definition "relationship between a model and a signature (vocabulary) such that the model provides a semantic interpretation of all non-logical symbols in the signature"@en
    
    Domain: 
        Model
    
    Range: 
        Signature
    SubPropertyOf: isMathematicallyRelatedTo
    
    
ObjectProperty: satisfies
    Annotations: 
        skos:definition "relationship between a model and a sentence indicating that the sentence holds true in the model"@en,
        dct:abstract ""@en,
        rdfs:label "satisfies"@en,
        rdfs:seeAlso SatisfactionRelation
    
    Domain: 
        Model
    
    Range: 
        Sentence
    SubPropertyOf: isMathematicallyRelatedTo
    
    
ObjectProperty: isMappedBy
    Annotations:
        rdfs:comment "The object mapping maps from the subject into something of the same type as the subject."@en, 
        rdfs:label "is mapped by"@en
    
    InverseOf: 
        mapsFrom
    
    SubPropertyOf: isRelatedAsPartOfMapsTo	
    
    
ObjectProperty: extendsTo
    Annotations: 
        rdfs:comment "The subject is a mapping of an extension, the object is the target of the extension mapping, i.e. the extended OMS."@en,
        rdfs:label "extends to"@en
    
    SubPropertyOf: 
        mapsTo
    
    Domain: 
        ExtensionMapping
    
    Range: 
        OMS
    SubPropertyOf: isLinguisticallyRelatedTo
    
    
    
ObjectProperty: isFormalizedBy
    Annotations: 
        rdfs:label "is formalized by"@en,
        rdfs:comment "The object is a precise mathematical entity capturing the subject (which is an informal or semi-formal entity)"@en
    
    InverseOf: 
        formalizes
    SubPropertyOf: isSemanticallyRelatedTo
    
    
ObjectProperty: isApproximantOf
    Annotations: 
        skos:definition "approximation (in the sense of a logically implied theory, possibly aftersuitable translation) of an OMS in a smaller signature or OMS language"@en,
        rdfs:label "is approximant of"@en
    
    Characteristics: 
        Transitive
    
    Domain: 
        OMS
    
    Range: 
        OMS
    SubPropertyOf: isEntailedBy
    
    
    
    
ObjectProperty: isModuleOf
    Annotations: 
        skos:definition "relationship between two OMS where the first conservatively extends to the second OMS"@en,
        rdfs:label "is module of"@en
    
    SubPropertyOf: 
        isSubOMSOf
    
    InverseOf: 
        isConservativeExtensionOf
    SubPropertyOf: isLogicallyRelatedTo
    
    
ObjectProperty: hasPart
    Annotations: 
        rdfs:label "has part"@en,
        skos:definition "relationship between two things were the second is a component of the first"@en
    
    
Class: OMSNetwork

    Annotations: 
        skos:note "An OMS network is a diagram of OMS in the sense of category theory, but different from a diagram in the sense of model-driven architecture."@en,
        skos:definition "collection of named OMS, possibly written in different OMS languages, linked by named OMS mappings and named OMS networks"@en,
        skos:note "collection is used here in the sense of syntactic collection"@en,
        skos:altLabel "hyperontology"@en,
        rdfs:label "OMS network"@en
    
    SubClassOf: 
        DOLEntity
	

    
Class: SequenceOfCorrespondences
    Annotations: 
        skos:definition "sequence whose members are correspondences."@en,
         skos:note "sequence is used here in the sense of syntactic sequence"@en,
       rdfs:label "sequence of correspondences"@en
    
    SubClassOf: DOLEntity
    
    
Class: LanguageMapping

    Annotations: 
        rdfs:label "language mapping"@en,
        skos:definition "mapping between languages"@en
    
    EquivalentTo: 
        (mapsFrom exactly 1 Language)
         and (mapsTo exactly 1 Language)
    
    SubClassOf: 
        Mapping
    
DisjointClasses:
        LanguageMapping, LogicMapping, OMSMapping

Class: SetOfMappings

    Annotations: 
        skos:definition "set whose members are mappings."@en,
        rdfs:label "set of mappings"@en
    
    SubClassOf: 
        Set
    
    
Class: DefinitionalExtensionMapping

    Annotations: 
	rdfs:label "definitional extension mapping"@en,
        skos:note "Each definitional extension is also a monomorphic extension but not vice versa."@en,
        skos:note "An extension $O_2$ of an OMS $O_1$ is a definitional extension, if each model of $O_1$ can be uniquely expanded to a model of $O_2$."@en,
        rdfs:label "definitional extension mapping"@en,
        skos:definition "extension whose newly introduced non-logical symbols are interpreted in a unique way"@en,
        skos:note "$O_2$ being a definitional extension of $O_1$ implies a bijective correspondence between the classes of models of $O_2$ and $O_1$."@en,
        reifies isDefinitionalExtensionOf
    
    EquivalentTo: 
        ModelTheoreticConservativeExtensionMapping
         and WeakDefinitionalExtensionMapping
    
    SubClassOf: 
        MonomorphicExtensionMapping
    
    
Class: LogicalLanguageAspect

    Annotations: 
        skos:definition "the (unique) language aspect of an OMS language that enables the expression of non-logical symbols and sentences in a logical language"@en,
        rdfs:label "logical language aspect"@en
    
    SubClassOf: 
        LanguageAspect
    
DisjointClasses:
        LogicalLanguageAspect,StructuringLanguageAspect, AnnotationExpressionLanguageAspect

Class: SetOfNonlogicalSymbols

    Annotations: 
        skos:definition "set whose members are non-logical symbols"@en,
        rdfs:label "set of non-logical symbols"@en
    
    SubClassOf: 
        CollectionOfExpressions
    
    
Class: ModelTheoreticConservativeExtensionMapping

    Annotations: 
        rdfs:label "model-theoretic conservative extension mapping"@en,
        skos:note "Any model-theoretic conservative extension is also a consequence-theoretic one."@en,
        skos:definition "extension mapping that does not lead to a restriction of class of models of an OMS"@en,
        skos:note "An extension $O_2$ of an OMS $O_1$ is a model-theoretic conservative extension, if all properties formulated in the signature of $O_1$ hold for $O_1$ whenever they hold for $O_2$."@en,
        reifies isModelTheoreticallyConservativeExtensionOf
    
    SubClassOf: 
        ConservativeExtensionMapping
    
    
Class: QueryVariable

    Annotations: 
        skos:note "If there are no variables in an OMS language, constants can be used as query variables."@en,
        skos:definition "symbol that will be used in a query and a substitution"@en,
        skos:note "Usually, query variables are the free variables of a sentence, whereas there can be other (bound) variables."@en,
        skos:note "From an abstract point of view, query variables are just symbols; they are used in a way that they will be substituted using a substitution. Many OMS languages have special notations for (query) variables."@en,
        rdfs:label "query variable"@en
    
    SubClassOf: 
        NonLogicalSymbol
    
    
Class: ModuleExtraction

    Annotations: 
	rdfs:label "module extraction"@en,
        sm:informativeReference "Cited and slightly adapted from \\cite{SuarezFigueroaEtAl:OntologyGlossary2008}"@en,
        rdfs:label "module extraction"@en,
        skos:definition "activity of obtaining from an OMS concrete modules to be used for a particular purpose (e.g. to contain a particular sub-signature of the original OMS)"@en,
        skos:note "The goal of module extraction is ``decomposing an OMS into smaller, more manageable modules with appropriate dependencies'' \\cite{DBLP:series/lncs/5445}"@en
    SubClassOf: Process
    
	
Class: ModuleExtractor
    Annotations: 
	rdfs:label "module extractor"@en,
	skos:definition "tool that implements module extraction"@en
    SubClassOf: Tool, hasProficiency some ModuleExtraction
    
Class: StandoffMarkup
    Annotations: 
        skos:definition "way of providing annotations to subjects in external resources, without embedding them into the original resource (here: OMS)"@en,
        rdfs:label "standoff markup"@en
    
    SubClassOf: 
        Language
    
    
Class: SequenceOfOMS
    Annotations: 
        rdfs:label "sequence of OMS"@en,
        skos:definition "sequence whose members are OMS."@en,
        skos:note "sequence is used here in the sense of syntactic sequence"@en
    SubClassOf: 
        DOLEntity
    
    
    
Class: MonomorphicExtensionMapping
    Annotations: 
        skos:note "Each monomorphic extension is also a model-theoretic conservative extension but not vice versa."@en,
        rdfs:label "monomorphic extension mapping"@en,
        skos:note "An extension $O_2$ of an OMS $O_1$ is a monomorphic extension, if each model of $O_1$ can be expanded to a model of $O_2$ that is unique up to isomorphism."@en,
        skos:definition "extension whose newly introduced non-logical symbols are interpreted in a way unique up to isomorphism"@en,
        reifies isMonomorphicExtensionOf
    
    SubClassOf: 
        ModelTheoreticConservativeExtensionMapping
    
    
Class: SetOfSentences
    Annotations: 
        skos:definition "set whose members are sentences"@en,
        rdfs:label "set of sentences"@en
    
    SubClassOf: 
        Set
    
    
Class: Institution
    Annotations: 
        skos:definition "metaframework mathematically formalising the notion of a logic"@en,
        rdfs:label "institution"@en
    
    SubClassOf: 
        formalizes some Logic, hasPart some Signature, hasPart some SignatureMorphism, hasPart some Model, hasPart some Sentence, hasPart some SatisfactionRelation, hasPart some Category
        SubClassOf: MathematicalEntity

    
    
Class: Signature
    Annotations: 
        skos:note "The signature of a term is the set of all non-logical symbols occuring in the term. The signature of an OMS language is the set of all non-logical symbols possible in that language."@en,
        rdfs:label "signature"@en,
        skos:definition "set (or otherwise structured entity) of non-logical symbols of an OMS"@en
    
    SubClassOf: 
        hasPart some SetOfNonlogicalSymbols, MathematicalEntity
    
    
Class: AxiomSentence
    Annotations: 
        skos:definition "sentence postulated to be valid (i.e.\\ true in every model)"@en,
        rdfs:label "axiom sentence"@en
    
    SubClassOf: 
        Sentence
    
    
Class: LogicalTheory
    Annotations: 
        rdfs:label "logical theory"@en,
        skos:definition "signature equipped with a set of sentences over the signature"@en,
        skos:note "The sentences must use only those non-logical symbols that are present in the signature."@en
    
    SubClassOf: 
        hasPart exactly 1 SetOfSentences,
        hasPart exactly 1 Signature
    SubClassOf: MathematicalEntity
    
    
Class: FlattenableOMS
    Annotations: 
        rdfs:label "flattenable OMS"@en,
        skos:note "More precisely, an OMS is flattenable if and only if it is either a basic OMS or it is an extension, union, translation, module extraction, approximation, filtering, or reference of named OMS involving only flattenable OMS."@en,
        skos:definition "OMS that can be seen, by purely syntactical means, to be logically equivalent to a basic OMS"@en
    
    SubClassOf: 
        OMS
    
    DisjointWith: 
        ElusiveOMS
    
    
    
Class: HomogeneousOMS
    Annotations: 
        skos:definition "OMS whose parts are supported by one logic"@en,
        rdfs:label "homogeneous OMS"@en
    
    SubClassOf: 
        OMS
    
    DisjointWith: 
        HeterogeneousOMS
    
    
Class: NonLogicalSymbol
    Annotations: 
        skos:definition "atomic expression or syntactic constituent of an OMS that requires an interpretation through a model"@en,
        rdfs:comment "a non-logical symbol in an OMS"@en,
        skos:example "Non-logical symbols in OWL \\nisref{W3C/TR REC-owl2-syntax:2009} (there called ``entities'') comprise \\begin{itemize} \\item individuals (denoting objects from the domain of discourse), \\item classes (denoting sets of objects; also called concepts), and \\item properties (denoting binary relations over objects; also called roles). \\end{itemize} This is opposed to logical symbols in OWL, e.g.\\ those for intersection and union of classes. "@en,
        skos:note "The notion of ``atomic sentence'' used in logic is different, it usually may involve several non-logical symbols. "@en,
        rdfs:label "non-logical symbol"@en,
        skos:example " Non-logical symbols in Common Logic \\nisref{ISO/IEC 24707:2007} comprise \\begin{itemize} \\item names (denoting objects from the domain of discourse), \\item sequence markers (denoting sequences of objects). \\end{itemize} This is opposed to logical symbols in Common Logic, e.g.\\ logical connectives and quantifiers."@en,
        skos:altLabel "OMS symbol"@en
    
    SubClassOf: 
        Term
    
    
    
Class: Set
    Annotations: 
        skos:definition "set whose members have a certain type, as specified by the type parameter."@en,
        rdfs:label "set"@en
    SubClassOf: MathematicalEntity
	


Class: ImpliedExtensionMapping
    Annotations: 
        skos:note "A conservative extension $O_2$ of an OMS $O_1$ is an implied extension, if and only if the signature of $O_2$ is the signature of $O_1$. $O_2$ is an implied extension of $O_1$ if and only if the model class of $O_2$ is the model class of $O_1$."@en,
        skos:definition "model-theoretic conservative extension that does not introduce new non-logical symbols"@en,
        skos:note "Each implied extension is also a definitional extension but not vice versa."@en,
        rdfs:label "implied extension mapping"@en,
        reifies isImpliedExtensionOf
    
    SubClassOf: 
        DefinitionalExtensionMapping
    
Class: StructuredOMS
    Annotations: 
        skos:definition "OMS that results from other OMS by import, union, combination, renaming or other structuring operations"@en,
        rdfs:label "structured OMS"@en
    
    SubClassOf: 
        OMS
    
    
Class: Model
    Annotations: 
        skos:note "A model of an OMS is a model of the signature of the OMS that also satisfies all the additional constraints expressed by the OMS. In case of flattenable OMS, these constraints are expressed by the axioms of the OMS."@en,
        rdfs:label "model"@en,
        skos:scopeNote "This term is not to be confused with model (here called MDEModel) in the sense of modeling (i.e., the ``M'' in OMS)."@en,
        skos:definition " semantic interpretation of all non-logical symbols of a signature"@en
   
    SubClassOf: 
        isModelOfSignature some Signature
    SubClassOf: MathematicalEntity
    
    
Class: StructuringLanguageAspect
    Annotations: 
        skos:definition "the (unique) language aspect of an OMS language that covers structured OMS as well as the relations of basic OMS and structured OMS to each other, including, but not limited to imports, OMS mappings, conservative extensions, and the handling of prefixes for CURIEs"@en,
        rdfs:label "structuring language aspect"@en
    
    SubClassOf: 
        LanguageAspect

    
Class: AnswerSubstitution
    Annotations: 
        skos:definition "substitution that, when applied to a given query, turns the latter into a logical consequence of a given OMS"@en,
        rdfs:label "answer substitution"@en
    
    SubClassOf: 
        Substitution
    
    
Class: Substitution
    Annotations: 
        rdfs:label "substitution"@en,
        skos:definition "OMS mapping that maps query variables of one OMS to complex terms of another OMS"@en
    
    SubClassOf: 
        OMSMapping
    
    
Class: SatisfactionRelation
    Annotations: 
        rdfs:label "satisfaction relation"@en,
        rdfs:seeAlso satisfies,
        skos:definition "relation between models and sentences indicating which sentences hold true in the model"@en
    SubClassOf: MathematicalEntity
    
    
Class: ConservativeExtensionMapping
    Annotations: 
        skos:definition "extension mapping of a consequence-theoretic or model-theoretic conservative extension"@en,
        rdfs:label "conservative extension mapping"@en,
        skos:note "If used without qualification, the consequence-theoretic version is meant."@en,
        reifies isConservativeExtensionOf
    
    SubClassOf: 
        ExtensionMapping
    
    
    
Class: HeterogeneousEnvironment
    Annotations: 
        rdfs:label "heterogeneous environment"@en,
        skos:definition "environment for the expression of homogeneous and heterogeneous OMS, comprising a logic graph, an OMS language graph and a supports relation"@en
    
    SubClassOf: 
        hasPart some LanguageGraph,
        hasPart some LogicGraph,
        hasPart some SupportsRelation
        SubClassOf: MathematicalEntity

    
Class: LanguageAspect
    Annotations: 
        skos:definition "set of language constructs of a given language, not necessarily forming a sublanguage"@en,
        rdfs:label "language aspect"@en
    SubClassOf: LinguisticEntity
    
    
    
    
    
Class: Profile
    Annotations: 
        skos:note "Profiles typically correspond to sublogics. "@en,
        skos:definition "(syntactic) sublanguage of an OMS language interpreting according to a particular logic that targets specific applications or reasoning methods} "@en,
        skos:note " Profiles can have different logics, even with completely different semantics, e.g.\\ OWL 2 DL versus OWL 2 Full."@en,
        skos:note " The logic needs to support the language. "@en,
        skos:example "Profiles of OWL 2 include OWL 2 EL, OWL 2 QL, OWL 2 RL, OWL 2 DL, and OWL 2 Full."@en,
        rdfs:label "profile"@en
    
    SubClassOf: 
        supportsLogic some Logic,
        OMSLanguage
    
    
Class: ExtensionMapping
    Annotations: 
        skos:definition "mapping between two OMS where the sets of non-logical symbols and sentences of the second OMS are supersets of those present in the first OMS"@en,
        rdfs:label "extension mapping"@en,
        skos:editorialNote "This definition differs from that in the Terms and Definition section of the DOL specification by focussing on the mapping rather than the codomain of the mapping."@en
    
    SubClassOf: 
        OMSMapping
    
    
Class: OMSDocumentation
    Annotations: 
        skos:definition "set of all annotations to an OMS, plus any other documents and explanatory comments generated during the entire OMS building process"@en,
        rdfs:label "OMS documentation"@en,
        sm:informativeReference "Adapted from \\cite{SuarezFigueroaEtAl:OntologyGlossary2008}"@en
    SubClassOf: LinguisticEntity
    
    
Class: SupportsRelation
    Annotations: 
        rdfs:label "supports relation"@en,
        skos:definition "relation between OMS languages and logics expressing the logical language aspect of the former, namely that the constructs of the former lead to a logical theory in the latter."@en,
	skos:note "There is also a supports relation between OMS languages and serializations, and one between language mappings and logic mappings."@en,
        reifies supportsLogic,
        reifies supportsSerialization,
        reifies supportsLogicMapping
    SubClassOf: SemanticEntity

ObjectProperty: supportsLogicMapping
    Annotations: 
	rdfs:label "supports logic mapping"@en,
        rdfs:comment "The subject language mapping corresponds to the object logic mapping."@en
    
    Domain: 
        OMSLanguageTranslation
    
    Range: 
        LogicMapping
    SubPropertyOf: isSemanticallyRelatedTo
    
    
Class: SetOfAnnotationExpressions
    Annotations: 
        rdfs:label "set of annotation expressions"@en,
        skos:definition "set whose members are annotation expressions."@en
    
    SubClassOf: 
        CollectionOfExpressions
    
    
Class: ElusiveOMS
    Annotations: 
        skos:definition "OMS that is not flattenable"@en,
        rdfs:label "elusive OMS"@en
    
    SubClassOf: 
        OMS
    
    DisjointWith: 
        FlattenableOMS
    
	
Class: WeakDefinitionalExtensionMapping
    Annotations: 
        skos:note "An extension is definitional if and only if it is both weakly definitional and model-theoretically conservative."@en,
        skos:definition "extension whose newly introduced non-logical symbols can be interpreted in at most one way"@en,
        rdfs:label "weak definitional extension mapping"@en,
        skos:note "An extension $O_2$ of an OMS $O_1$ is a weak definitional extension, if each model of $O_1$ can be expanded to at most one model of $O_2$."@en,
        reifies isWeakDefinitionalExtensionOf
    
    SubClassOf: 
        ExtensionMapping
    
    
Class: TheoremSentence
    Annotations: 
        rdfs:label "theorem sentence"@en,
        skos:definition "sentence that has been proven from other axioms and theorems"@en
    
    SubClassOf: 
        Sentence
    
    
Class: Mapping
    Annotations: 
        reifies isMappableTo,
        rdfs:comment "a generic mapping (translation or reduction)"@en,   
        skos:definition "relation between a set of inputs and a set of permissible outputs with the property that each input is related to exactly one output."@en,
        rdfs:label "mapping"@en,
        skos:note "alternative term: function"@en,
        skos:note "in some cases is a morphism, as in Category Theory."@en	
    EquivalentTo: 
        (mapsFrom exactly 1 owl:Thing)
         and (mapsTo exactly 1 owl:Thing)
    SubClassOf: MathematicalEntity
    
    
Class: AnnotationExpressionLanguageAspect
    Annotations: 
        skos:definition "the (unique) language aspect of an OMS language that enables the expression of comments and annotations"@en,
        rdfs:label "annotation expression language aspect"@en
    
    SubClassOf: 
        LanguageAspect

Class: Term
    Annotations: 
        skos:definition "syntactic expression either consisting of a single non-logical symbol or recursively composed of other terms (a.k.a. its subterms)"@en,
        rdfs:label "term"@en
    
    SubClassOf: 
        Expression
    
    
Class: ConsequenceTheoreticConservativeExtensionMapping
    Annotations: 
        skos:definition "extension that does not add new theorems (in terms of the unextended signature)"@en,
        rdfs:label "consequence-theoretic conservative extension mapping"@en,
        skos:note "An extension $O_2$ of an OMS $O_1$ is a consequence-theoretic conservative extension, if all properties formulated in the signature of $O_1$ hold for $O_1$ whenever they hold for $O_2$."@en,
        reifies isConsequenceTheoreticallyConservativeExtensionOf
    
    SubClassOf: 
        ConservativeExtensionMapping
    
    
Class: Resource
    Annotations: 
        skos:example "Familiar examples include an electronic document, an image, a source of information with a consistent purpose (e.g., ``today's weather report for Los Angeles''), a service (e.g., an HTTP-to-SMS gateway), and a collection of other resources. A resource is not necessarily accessible via the Internet; e.g., human beings, corporations, and bound books in a library can also be resources. Likewise, abstract concepts can be resources, such as the operators and operands of a mathematical equation, the types of a relationship (e.g., ``parent'' or ``employee''), or numeric values (e.g., zero, one, and infinity). \\nisref{IETF/RFC 3986:2005, Section 1.1}"@en,
        skos:definition "something that can be globally identified"@en,
        skos:note "\\nisref{IETF/RFC 3986:2005, Section 1.1} deliberately defines a resource as ``in a general sense \\textelp{} whatever might be identified by \\textins*{an IRI}''. The original source refers to URIs, but DOL uses the compatible IRI standard \\nisref{IETF/RFC 3987:2005} for identification."@en,
        rdfs:label "resource"@en
    SubClassOf: WebEntity    
    
Class: LogicGraph
    Annotations: 
        skos:definition "graph of logics, logic translations and logic reductions, typically used in a heterogeneous environment."@en,
        skos:note "In a logic graph, some of the logic translations and reductions can be marked to be default translations."@en,
        rdfs:label "logic graph"@en
    
    SubClassOf: 
        Graph
    
Class: Approximation
    Annotations: 
	rdfs:label "approximation"@en,
	skos:definition "structured OMS that expresses a maximum approximant."@en
    SubClassOf: DOLStructuredOMS, hasPart some DOLStructuredOMS
	    
    
Class: QueryLanguage
    Annotations: 
        skos:scopeNote " There are also general purpose OMS languages, which can express both OMS and quries."@en,
        skos:definition "OMS language specifically dedicated to queries"@en,
        rdfs:label "query language"@en,
        skos:example " SPARQL, Prolog "@en
    
    SubClassOf: 
        OMSLanguage
    
    
Class: Query
    Annotations: 
        skos:definition "sentence containing query variables that can be instantiated by a substitution"@en,
        rdfs:label "query"@en
    
    SubClassOf: 
        Sentence
    
    
Class: LanguageGraph
    Annotations: 
        rdfs:label "OMS language graph"@en,
        skos:definition "graph of OMS languages and OMS language translations, typically used in a heterogeneous environment."@en
    
    SubClassOf: 
        Graph
    
    
Class: HeterogeneousOMS
    Annotations: 
        skos:definition "OMS whose parts are supported by different logics"@en,
        rdfs:label "heterogeneous OMS"@en
    
    SubClassOf: 
        OMS
    
    DisjointWith: 
        HomogeneousOMS
    
    
    
Class: Equivalence
    Annotations: 
        skos:definition "OMS mapping ensuring that two OMS share the same definable concepts"@en,
        rdfs:label "equivalence"@en,
        skos:note " Two OMS are equivalent if they have a common definitional extension. The OMS may be written in different OMS languages. "@en
    
    SubClassOf: 
        OMSMapping
    
    
    
Class: LinkedData
    Annotations: 
        skos:definition "structured data that is published on the Web in a machine-processable way, according to principles explained in http://linkeddata.org/"@en,
        skos:note " The linked data principles (adapted from \\cite{BernersLee:LinkedData2006} and its paraphrase at \\cite{Wikipedia:LinkedData2011}) are the following: \\begin{enumerate} \\item Use IRIs as names for things. \\item Use HTTP IRIs so that these things can be referred to and looked up (``dereferenced'') by people and user agents.\\footnote{I.e., the IRI is treated as a URL (uniform resource locator).} \\item Provide useful machine-processable (plus optionally human-readable) information about the thing when its IRI is dereferenced, using standard formats. \\item Include links to other, related IRIs in the exposed data to improve discovery of other related information on the Web. \\end{enumerate} "@en,
        rdfs:label "linked data"@en,
        skos:note " RDF, serialized as RDF/XML \\cite{W3C:REC-rdf-syntax-grammar-20040210}, is the most common format for publishing linked data. However, its usage is not mandatory. "@en,
        skos:note " Using HTTP content negotiation \\cite{rfc2616} it is possible to serve representations in different formats from the same URL. "@en
    
    SubClassOf: WebEntity    
    
    
Class: LogicTranslation
    Annotations: 
        rdfs:label "logic translation"@en,
        skos:definition "translation of a source logic into a target logic (mapping signatures, sentences and models) that keeps or encodes the logical content of OMS"@en,
	skos:note "mapping between logics representing all structure, in contrast to reduction"@en
    SubClassOf: 
        LogicMapping
    
    
Class: Graph
    Annotations: 
        skos:definition "set of objects (nodes) that are connected by links (edges)"@en,
        rdfs:label "graph"@en,
        skos:altLabel "network"@en
    SubClassOf: MathematicalEntity
    
    
Class: CollectionOfExpressions
    Annotations: 
        rdfs:label "collection of expressions"@en,
        skos:definition "collection whose members are expressions"@en
    SubClassOf: LinguisticEntity
    
    
    
Class: LogicReduction
    Annotations: 
        skos:definition "reduction of a source logic onto a (usually less expressive) target logic (mapping signatures, sentences and models) that simply forgets those parts of the logical structure not fitting the target logic"@en,
	skos:note "mapping between logics forgetting parts of the structure, projection to a smaller logic, in contrast to reduction"@en,
        rdfs:label "logic reduction"@en
    
    SubClassOf: 
        LogicMapping
    
    
Class: Expression
    Annotations: 
        skos:definition "a finite combination of symbols that are well-formed according to applicable rules (depending on the language)"@en,
        rdfs:label "expression"@en
    
    SubClassOf: 
        usesLanguage exactly 1 Language
    SubClassOf: LinguisticEntity
    
    
    
Class: AnnotationExpression
    Annotations: 
        skos:definition "additional information without a logical semantics that is attached to an element of an OMS"@en,
        skos:note "\\label{note:annotation-rdf} Formally, an annotation is given as a $(\\text{subject}, \\text{predicate}, \\text{object})$ triple as defined by \\nisref{SOURCE: W3C/TR REC-rdf-concepts:2004, Section 6}. The subject of an annotation is an element of an OMS. The predicate is an RDF property defined in an external OMS and describes in what way the annotation object is related to the annotation subject. "@en,
        skos:note " According to note~\\ref{note:annotation-rdf} it is possible to interpret annotations under an RDF semantics. ``Without a logical semantics'' in this definition means that annotations to an OMS are not considered sentences of that OMS. "@en,
        rdfs:label "annotation expression"@en
    
    SubClassOf: 
        Expression
    
    
Class: OMSTranslation
    Annotations: 
        rdfs:label "OMS translation"@en,
        skos:definition "DOL structured OMS expressing the assignment of new names to some non-logical symbols of an OMS, or translation of an OMS along a language translation"@en,
        skos:note " An OMS translation results in an OMS mapping between the original and the translation OMS. "@en
    
    SubClassOf: 
        DOLStructuredOMS, hasPart some DOLStructuredOMS
    
    
Individual: DOL

    Annotations: 
        skos:note "When viewed as an OMS language, DOL has OMS as its non-logical symbols, and OMS mappings as its sentences."@en,
        rdfs:label "Distributed Ontology, Model and Specification Language"@en,
        skos:definition "unified metalanguage for the structured and heterogeneous expression of ontologies, specifications, and models, using DOL libraries of OMS, OMS mappings and OMS networks"@en
    
    Types: 
        OMSLanguage
    
Class: AbstractSyntax
Annotations: 
        skos:note "An abstract syntax can be specified as a MOF metamodel. Then abstract abstract syntax documents can be represented as  XMI documents."@en,
        rdfs:label "abstract syntax"@en,
        skos:definition	"term language for representing documents in a machine-processable way"@en
    SubClassOf: LinguisticEntity
	
Class: Category
Annotations: 
	rdfs:label "category"@en,
        skos:definition "a class of objects with suitable morphisms between them"@en,
        skos:note "In DOL, objects of a category are usually signatures or OMS, and morphisms are signature morphisms, or OMS mappings. In principle, no assumption about the exact nature of objects and morphisms is made."@en,
        skos:note "The morphisms determine which part of the structure of the objects is relevant, i.e. preserved by morphisms. Hence, objects can be seen as 'sets with structure', and morphisms as 'structure-preserving maps'.  However note that not all categories can be obtained in this way."@en
    SubClassOf: MathematicalEntity
	
	
Class: Closure
Annotations: 
	rdfs:label "closure"@en,
        skos:definition "structured OMS expressing a variant of the closed world assumption by restricting the models to those that are minimal or maximal (with respect to the local environment). The closed world assumption is a default assumption about facts whose status in unknown."@en,
        skos:note "Symbols from the local environment are assumed to have a fixed interpretation. Only the symbols newly declared in the closure are forced to have minimal or maximal interpretation."@en,
        skos:note "DOL supports four different forms of closure: minimization and maximization as well as freeness and cofreeness."@en
        SubClassOf: DOLStructuredOMS, hasPart some DOLStructuredOMS
	
	
Class: Cofreeness
Annotations: 
	rdfs:label "cofreeness"@en,
        skos:definition "special type of closure, restriction of models to those that are cofree (with respect to the local environment)."@en,
        skos:note "In first-order-like logics, cofreeness means maximal interpretation of predicates and equality being observable equivalence. Cofreeness can be used for the specification of coinductive datatypes like infinite lists and streams."@en
    SubClassOf: Closure

Class: Freeness
Annotations: 
	rdfs:label "freeness"@en,
        skos:definition "special type of closure, restriction of models to those that are free (with respect to the local environment)."@en,
        skos:note "In first-order logic (and similar logics), freeness means minimal interpretation of predicates and minimal equality among data values. Freeness can be used for the specification of inductive datatypes like numbers, lists, trees, bags etc. In order to specify e.g. lists over some elements, the specification of the elements should be in the local environment."@en
    SubClassOf: Closure
	
Class: Minimization
    Annotations: 
	rdfs:label "minimization"@en,
        skos:definition "form of closure that restricts the models to those that are minimal (with respect to the local environment)."@en,
        skos:note "Also known as circumscription."@en
    SubClassOf: Closure

Class: Maximization
    Annotations: 
	rdfs:label "maximization"@en,
	skos:definition "form of closure that restricts the models to those that are maximal (with respect to the local environment)."@en
    SubClassOf: Closure
	
Class: Union
    Annotations: 
	rdfs:label "union"@en,
        skos:definition "structured OMS expressing the combination of all symbols and axioms (and more general constraints) of a sequence of OMS"@en
    SubClassOf: DOLStructuredOMS, hasPart some DOLStructuredOMS
	
Class: Extension
    Annotations: 
	rdfs:label "extension"@en,
	skos:definition "structured OMS extending a given OMS with new symbols and sentences."@en,
        skos:note "The new symbols and sentences are interpreted relative to the
local envorinment, which is the signature of the 'given OMS'."@en
    SubClassOf: DOLStructuredOMS, hasPart some DOLStructuredOMS
	
Class: ConservativeExtension
    Annotations: 
	skos:definition "extension that does not add new logical properties with respect to the signature of the extended OMS."@en,
        rdfs:label "conservative extension"@en
    SubClassOf: Extension
	
	
Class: ConsequenceTheoreticConservativeExtension
    Annotations: 
        rdfs:label "consequence-theoretic conservative extension"@en,
	skos:definition "extension that does not add new theorems (in terms of the unextended signature)."@en,
        skos:note "An extension $O_2$ of an OMS $O_1$ is a consequence-theoretic conservative extension, if all properties formulated in the signature of $O_1$ hold for $O_1$ whenever they hold for $O_2$."@en
    SubClassOf: ConservativeExtension


Class: ModelTheoreticConservativeExtension
    Annotations: 
        rdfs:label "model-theoretic conservative extension"@en,
	skos:definition "extension that does not lead to a restriction of class of models of an OMS."@en,
        skos:note "An extension $O_2$ of an OMS $O_1$ is a model-theoretic conservative extension, if all properties formulated in the signature of $O_1$ hold for $O_1$ whenever they hold for $O_2$."@en
    SubClassOf: ConservativeExtension
	

Class: MonomorphicExtension
    Annotations: 
        rdfs:label "monomorphic extension"@en,
	skos:definition "extension whose newly introduced non-logical symbols are interpreted in a way unique up to isomorphism."@en,
        skos:note "An extension $O_2$ of an OMS $O_1$ is a monomorphic extension, if each model of $O_1$ can be expanded to a model of $O_2$ that is unique up to isomorphism."@en
    SubClassOf: ModelTheoreticConservativeExtension

Class: DefinitionalExtension
    Annotations: 
        rdfs:label "definitional extension"@en,
	skos:definition "extension whose newly introduced non-logical symbols are interpreted in a unique way."@en,
        skos:note "An extension $O_2$ of an OMS $O_1$ is a definitional extension, if each model of $O_1$ can be uniquely expanded to a model of $O_2$."@en
    SubClassOf: MonomorphicExtension
    EquivalentTo: ModelTheoreticConservativeExtension and WeakDefinitionalExtension


Class: WeakDefinitionalExtension
    Annotations: 
        rdfs:label "weak definitional extension"@en,
	skos:definition "extension whose newly introduced non-logical symbols can be interpreted in at most one way."@en,
        skos:note "An extension $O_2$ of an OMS $O_1$ is a weak definitional extension, if each model of $O_1$ can be expanded to at most one model of $O_2$."@en
    SubClassOf: Extension
	
Class: ImpliedExtension
    Annotations: 
        rdfs:label "implied extension"@en,
	skos:definition "model-theoretic conservative extension that does not introduce new non-logical symbols."@en,
        skos:note "A conservative extension $O_2$ of an OMS
    $O_1$ is an implied extension, if and only if the signature of
    $O_2$ is the signature of $O_1$.  $O_2$ is an implied extension of
    $O_1$ if and only if the model class of $O_2$ is the model class
    of $O_1$."@en
    SubClassOf: DefinitionalExtension
	

Class: ConsistentOMS
    Annotations: 
	rdfs:label "consistent OMS"@en,
	skos:definition "OMS that has a non-trivial set of logical consequences in the sense that not every sentence follows from the OMS."@en
    SubClassOf: OMS
    EquivalentTo: OMS and not InconsistentOMS	
	
Class: InconsistentOMS
    Annotations: 
	rdfs:label "inconsistent OMS"@en,
	skos:definition "OMS that has a trivial set of logical consequences in the sense that every sentence follows from the OMS."@en
    SubClassOf: UnsatisfiableOMS
    EquivalentTo: OMS and not ConsistentOMS	

Class: SatisfiableOMS
    Annotations: 
	rdfs:label "satisfiable OMS"@en,
	skos:definition "OMS that is satisfied by least one model."@en
    SubClassOf: ConsistentOMS
    EquivalentTo: OMS and not UnsatisfiableOMS	
	
Class: UnsatisfiableOMS
    Annotations: 
	rdfs:label "unsatisfiable OMS"@en,
	skos:definition "OMS that is not satisfied by any model."@en
    SubClassOf: OMS
    EquivalentTo: OMS and not SatisfiableOMS	
	
Class: ModelFinder
    Annotations:
        rdfs:label "model finder"@en,
	skos:definition "Tool that implements model finding"@en
    SubClassOf: Tool, hasProficiency some ModelFinding
	
Class: ModelFinding
    Annotations:
        rdfs:label "model finding"@en,
	skos:definition "process that finds models of an OMS and thus proves it to be satisfiable"@en
    SubClassOf: Process

Class: Module
    Annotations: 
	rdfs:label "module"@en,
	skos:definition "structured OMS expressing a subOMS that conservatively extends to conservative extension the whole OMS."@en
    SubClassOf: DOLStructuredOMS, hasPart some InterfaceSignature, hasPart some DOLStructuredOMS

Class: NativeOMS
    Annotations: 
        rdfs:label "native OMS"@en,
	skos:definition "sequence of expressions (like non-logical symbols, sentences and structuring elements) from a given OMS language."@en
    SubClassOf: OMS

Class: NativeDocument
    Annotations: 
        rdfs:label "native document"@en,
	skos:definition "document containing a native OMS."@en
    SubClassOf: Document
	
Class: DOLDocument
    Annotations: 
        rdfs:label "DOL document"@en,
	skos:definition "document containing a DOL library."@en
    SubClassOf: Document, DOLEntity
	
Class: Document
    Annotations: 
	rdfs:label "document"@en,
	skos:definition "result of serializing an OMS or DOL library using a given serialization."@en
    SubClassOf: LinguisticEntity
	
Class: Approximant
    Annotations: 
	rdfs:label "approximant"@en,
	skos:definition "approximation (in the sense of a logically implied theory, possibly after suitable translation)  of an OMS in a smaller signature or a sublanguage."@en
    SubClassOf: OMS
	
Class: MaximumApproximant
    Annotations: 
        rdfs:label "maximum approximant"@en,
	skos:definition "best possible (in the sense of a maximum set of logical consequences approximant of an OMS in a smaller signature or a sublanguage."@en,
        skos:note "Technically, a maximum approximant is a uniform interpolant"@en
    SubClassOf: Approximant
	
Class: Filtering
    Annotations: 
	rdfs:label "filtering"@en,
	skos:definition "structured OMS expressing the verbatim removal of symbols or axioms from an OMS."@en,
        skos:note "If a symbol is removed, all axioms containing that symbol are removed, too."@en
    SubClassOf: DOLStructuredOMS, hasPart some DOLStructuredOMS
	
Class: Tool
    Annotations: 
	rdfs:label "tool"@en,
	skos:definition "software for processing DOL libraries and OMS."@en

Class: Combination
    Annotations: 
	rdfs:label "combination"@en,	
        skos:example "Consider an ontology involving a concept Person, and another one involving Human being, and an alignment that relates these to concepts. In the combination of the ontologies along the alignment, there is only one concept, representing both Person and Human being."@en,
        skos:definition "structured OMS expressing the aggregation of all the OMS in an OMS network, where non-logical symbols are shared according to the OMS mappings in the OMS network "@en
    SubClassOf: DOLStructuredOMS, hasPart some OMSNetwork

Class: Correspondence
    Annotations: 
	rdfs:label "correspondence"@en,
	skos:definition "relationship between an non-logical symbol $e_1$ from an OMS $O_1$ and an non-logical symbol $e_2$ from an OMS $O_2$, or between an non-logical symbol $e_1$ from $O_1$ and a term $t_2$ formed from non-logical symbols\index{non-logical symbol from $O_2$."@en,
        skos:note "A correspondence is given as a quadruple 
$(e_1, R, e_2, c)$,
where $R$ denotes the type of relationship that is asserted to hold between the two non-logical 
symbols/terms, and 0<=c<=1 is a confidence value.  $R$ and $c$ may be omitted: When $R$ is 
omitted, it defaults to the equivalence relation, unless another default
relation has been explicitly specified; when $c$ is omitted, it defaults to 1."@en
    SubClassOf: DOLEntity
	
	
Class: DOLStructuredOMS
    Annotations: 
        rdfs:label "DOL structured OMS"@en,
	skos:definition "syntactically valid DOL expression denoting an OMS that is built from smaller OMS as building blocks."@en,
	skos:note "DOL structured OMS, typically, use basic OMS as building blocks for defining other structured OMS, OMS mappings or OMS networks."@en
    SubClassOf: StructuredOMS	
	
Class: Entailment
    Annotations: 
	rdfs:label "entailment"@en,
	skos:altLabel "logical consequence"@en,
	skos:definition "relation between two OMS (or an OMS and a sentence) expressing that the second one is logically implied by the first one."@en,
	skos:note "Entailment expresses that each model satisfying the first OMS also satisfies the second OMS (or the sentence, respectively)."@en,
	skos:note "Entailments can also be stated between networks, or networks and OMS."@en
    SubClassOf: OMSMapping	
	
Class: FormalSemantics
    Annotations: 
        rdfs:label "formal semantics"@en,
	skos:definition "assignment of a mathematical meaning to a language by mapping abstract syntax to suitable semantic domains"@en,
        skos:note "A formal semantics is a formalization of the meaning of a language."@en
    SubClassOf: hasPart some SemanticDomain, hasPart some SemanticRule,
        SemanticEntity, formalizes some Language	

Class: SemanticDomain
    Annotations: 
        rdfs:label "semantic domain"@en,
	skos:definition "mathematically-defined set of values that can represent the intended meanings of language constructs."@en
    SubClassOf: Set, SemanticEntity

Class: SemanticRule
    Annotations: 
        rdfs:label "semantic rule"@en,
	skos:definition "specification of a mapping from abstract syntax to a semantic domain."@en
    SubClassOf: SemanticEntity

Class: GlobalEnvironment
    Annotations: 
        rdfs:label "global environment"@en,
	skos:definition "mapping from identifiers (IRIs) to values in  semantics domains representing the global knowledge about OMS."@en
    SubClassOf: hasPart some LocalEnvironment
    SubClassOf: MathematicalEntity
	
Class: Import
    Annotations: 
	rdfs:label "import"@en,
	skos:definition "reference to an OMS behaving as if it were verbatim included; also import of DOL libraries."@en,
        skos:note "Semantically, an import of $O_2$ into $O_1$ is equivalent to the verbatim inclusion of $O_2$ in place of the import declaration."@en,
	skos:note "The purpose of $O_2$ importing $O_1$ is to make non-logical symbols and sentences of $O_1$ available in $O_2$."@en,
        skos:note "Importing $O_1$ into $O_2$ turns $O_2$ into an extension of $O_1$."@en,
        skos:note "The import of a whole DOL library into another DOL library is also called import."@en,
        skos:example "An owl:import in OWL is an import."@en
    SubClassOf: DOLStructuredOMS

Class: InterfaceSignature
    Annotations: 
        rdfs:label "interface signature"@en,
	skos:definition "signature mediating between an OMS and a module of that OMS in the sense that it contains those non-logical symbols that the sentences of the module and the sentences of the OMS have in common."@en
    SubClassOf: Signature
	
Class: LocalEnvironment
    Annotations: 
        rdfs:label "local environment"@en,
	skos:definition "signature built from all previously-declared symbols and axioms."@en
    SubClassOf: Signature
		
	
	
Class: Matching
    Annotations: 
	rdfs:label "matching"@en,
	skos:definition "algorithmic procedure that generates an alignment for two given OMS."@en
    SubClassOf: Process

Class: Matcher
    Annotations: 
	rdfs:label "matcher"@en,
	skos:definition "tool that implements matching"@en
    SubClassOf: Tool, hasProficiency some Matching
		
ObjectProperty: sharesWith
    Annotations: 
	rdfs:label "shares with"@en,
	skos:definition "property of OMS symbols being mapped to the same symbol when computing a combination of an OMS network."@en,
        skos:note "Sharing is always relative to a given OMS network that
  relates different OMS. That is, two given OMS symbols
  can share with respect to one OMS network, and not share with respect to some
  other OMS network."@en
    Domain: NonLogicalSymbol 
    Range: NonLogicalSymbol 
    SubPropertyOf: isLinguisticallyRelatedTo
	
	
Class: SignatureMorphism
    Annotations: 
        rdfs:label "signature morphism"@en,
	skos:definition "mapping between two signatures, preserving the structure of the source signature within the target signature"@en,
        skos:note "A list of symbol map items induces a signature morphism."@en
    SubClassOf: hasPart some SymbolMapItem
    SubClassOf: MathematicalEntity
	
	
Class: SymbolMapItem
    Annotations: 
        rdfs:label "symbol map item"@en,
	skos:definition "pair of symbols of two OMS, indicating how a symbol from the first OMS is mapped by a signature morphism to a symbol of the second OMS."@en,
        skos:note "A symbol map item is given as s_1 |-> s_2, where $s_1$ is a symbol from the source OMS and $s_2$ is a symbol from the target  of the OMS mapping."@en
    SubClassOf: hasPart some NonLogicalSymbol
    SubClassOf: DOLEntity
	
Class: TheoremProver
    Annotations: 
        rdfs:label "theorem prover"@en,
	skos:definition "software tool implementing theorem proving."@en
    SubClassOf: Tool, hasProficiency some TheoremProving
	
Class: TheoremProving
    Annotations: 
	rdfs:label "theorem proving"@en,
	skos:definition "process of demonstraing that a sentence (or OMS) is the logical consequence of some OMS."@en
    SubClassOf: Process
	
	
Class: LinguisticEntity
    Annotations: 
        rdfs:label "linguistic entity"@en,
	skos:definition "entity that is of linguistic, syntactic nature."@en

Class: DOLEntity
    Annotations: 
        rdfs:label "DOL entity"@en,
	skos:definition "entity that is used in DOL texts."@en

    SubClassOf: LinguisticEntity

Class: MathematicalEntity
    Annotations: 
        rdfs:label "mathematical entity"@en,
	skos:definition "entity that is part of a mathematical theory."@en

Class: SemanticEntity
    Annotations: 
        rdfs:label "semantic entity"@en,
	skos:definition "entity that is of semantic nature, i.e. relating linguistic objects with their semantic denotation in a mathematical structure."@en
	
Class: WebEntity
    Annotations: 
        rdfs:label "web entity"@en,
	skos:definition "entity that is related to the world wide web."@en
	
ObjectProperty: semanticallyDenotes
    Annotations: 
        rdfs:label "semantically denotes"@en,
	skos:definition "relation between a linguistic entity and its semantic denotation."@en
    Domain: LinguisticEntity
    Range: MathematicalEntity or SemanticEntity	
    SubPropertyOf: isSemanticallyRelatedTo	
	
ObjectProperty: isMathematicallyRelatedTo
    Annotations: 
        rdfs:label "is mathematically related to"@en,
	skos:definition "relation between mathematical entities."@en
    Domain: MathematicalEntity
    Range: MathematicalEntity	

ObjectProperty: isLinguisticallyRelatedTo
    Annotations: 
        rdfs:label "is linguistically related to"@en,
	skos:definition "relation between linguistic entities."@en
    Domain: LinguisticEntity
    Range: LinguisticEntity

ObjectProperty: isLogicallyRelatedTo
    Annotations: 
        rdfs:label "is logically related to"@en,
	skos:definition "relation between lingustic entities that has a logical, semantic nature."@en
    Domain: LinguisticEntity
    Range: LinguisticEntity
    SubPropertyOf: isSemanticallyRelatedTo	
	
	
ObjectProperty: isSemanticallyRelatedTo
    Annotations: 
        rdfs:label "is semantically related to"@en,
	skos:definition "relation that has a semantic nature."@en
    Domain: LinguisticEntity or MathematicalEntity or SemanticEntity
    Range: LinguisticEntity or MathematicalEntity or SemanticEntity
	
ObjectProperty: isRelatedAsPartOfMapsTo
    Annotations: 
        rdfs:label "is related as part of maps to"@en,
	skos:definition "property used in the context of mappings, for both linguistic and mathematical entities."@en

ObjectProperty:	hasProficiency
    Annotations: 
        rdfs:label "has proficiency"@en,
	skos:definition "property of a tool that is capable of implementing a process."@en
    Domain: Tool
    Range: Process
	
Class: Process
    Annotations: 
        rdfs:label "process"@en,
	skos:definition "algorithmic procedure working on DOL-related linguistic entities as input."@en
	
ObjectProperty: isImpliedExtensionOf
    Annotations: 
        strictlyStrongerThan isConservativeExtensionOf,
        skos:note "Each implied extension is also a definitional extension but not vice versa."@en,
        skos:definition "model-theoretic conservative extension that does not introduce new non-logical symbols"@en,
        skos:note " A conservative extension $O_2$ of an OMS $O_1$ is an implied extension, if and only if the signature of $O_2$ is the signature of $O_1$. $O_2$ is an implied extension of $O_1$ if and only if the model class of $O_2$ is the model class of $O_1$."@en,
        rdfs:label "is implied extension of"@en
    
    SubPropertyOf: 
        isDefinitionalExtensionOf
    
    SubPropertyChain: 
        isMappedBy o impliedExtendsTo
	
ObjectProperty: entails
    Annotations:
	rdfs:label "entails"@en,
	skos:definition "relation of logical entailment, expressing that all models of the subject are also models of the object"@en
    SubPropertyOf: isLogicallyRelatedTo	
    Domain: OMS or OMSNetwork
    Range: OMS or OMSNetwork or Sentence
	
ObjectProperty: isEntailedBy
    Annotations:
	rdfs:label "is entailed by"@en,
	skos:definition "inverse of relation of logical entailment"@en
    SubPropertyOf: isLogicallyRelatedTo	
    InverseOf: entails
    Domain: OMS or OMSNetwork or Sentence
    Range: OMS or OMSNetwork

	
Class: OMSSemanticObject
    Annotations:
	rdfs:label "OMS Semantic Object"@en,
        skos:definition "object giving the semantics of an OMS"@en
    SubClassOf: SemanticEntity, isMemberOf some SemanticDomain,
        hasLogic some Logic,
        hasSignature some Signature, 
	hasSentences some SetOfSentences, hasModels some ClassOfModels
	
Class: ClassOfModels
    Annotations:
	rdfs:label "class of models"@en,
        skos:definition "a class of models (over some signature in some logic)"@en
    SubClassOf: SemanticEntity

ObjectProperty: hasSignature
    Annotations:
	rdfs:label "has signature"@en,
        skos:definition "an OMS (resp. its semantic object) has an assoicated signature, which is the signature of the OMS"@en
    Domain: OMS or OMSSemanticObject 
    Range: Signature 
    SubPropertyOf: isSemanticallyRelatedTo
	
ObjectProperty: hasSentences
    Annotations:
rdfs:label "has sentences"@en,
        skos:definition "an OMS (resp. its semantic object) has an assoicated set of sentences, which is the set of sentences of the OMS"@en
    Domain: OMS or OMSSemanticObject 
    Range: SetOfSentences
    SubPropertyOf: isSemanticallyRelatedTo
	
ObjectProperty: hasModels
    Annotations:
	rdfs:label "has models"@en,
        skos:definition "an OMS (resp. its semantic object) has an assoicated class of models, which is the class of models of the OMS"@en
    Domain: OMS or OMSSemanticObject 
    Range: ClassOfModels
    SubPropertyOf: isSemanticallyRelatedTo	
	
Class: TranslationProcess
    Annotations:
	rdfs:label "translation (process)"@en,
	skos:definition "process of applying a language or logic translation, or flattening an OMS translation"@en
    SubClassOf: Process
	
Class: Flattening
    Annotations:
	rdfs:label "flattening"@en,
	skos:definition "process of transforming an OMS to an equivalent basic OMS"@en
    SubClassOf: Process
	
